EfficientChad.lean
@@ -1,1 +1,2 @@
 import EfficientChad.ChadCost
+import EfficientChad.Arrays
